Notationize everything! (broke some proper?)

coq/theories/OGS/Spec.v
@@ -47,7 +47,7 @@ TODO: concretize env
      1-5 : current status of the pdf
      6-10: administration
    *)
-  Record machine : Type := {
+  Class machine : Type := {
     (* configurations (used to be called "terms" far in the past)
        roughly: active states *)
     conf : ctx S.(typ) -> Type ;
@@ -62,100 +62,99 @@ TODO: concretize env
     v_sub {Γ Δ} : Γ =[val]> Δ -> val Γ ⇒ᵢ val Δ ;
     (* configuration substitution *)
     c_sub {Γ Δ} : Γ =[val]> Δ -> conf Γ -> conf Δ ;
-  }.
+    }.
 
-  Definition env (M : machine) Γ Δ := Γ =[M.(val)]> Δ.
+  Notation "u @ᵥ v" := (v_sub u _ v) (at level 30).
+  Notation "u @ₜ c" := (c_sub u c) (at level 30).
 
-  Definition v_ren {M Γ Δ} : Γ ⊆ Δ -> M.(val) Γ ⇒ᵢ M.(val) Δ :=
-    fun u => M.(v_sub) (s_ren M.(v_var) u) .
+  Context {M : machine}.
+ 
+  Notation "Γ ⇒ᵥ Δ" := (Γ =[val]> Δ) (at level 30).
+
+  Definition v_ren {Γ Δ} : Γ ⊆ Δ -> val Γ ⇒ᵢ val Δ :=
+    fun u => v_sub (v_var ⊛ᵣ u) .
       
-  Definition e_comp {M Γ1 Γ2 Γ3} (u : env M Γ2 Γ3) (v : env M Γ1 Γ2) : env M Γ1 Γ3
-    := s_map (M.(v_sub) u) v.
+  Definition e_comp {Γ1 Γ2 Γ3} : Γ2 ⇒ᵥ Γ3 -> Γ1 ⇒ᵥ Γ2 -> Γ1 ⇒ᵥ Γ3
+    := fun u v => s_map (v_sub u) v.
+  Infix "⊛" := e_comp (at level 14).
 
-  Definition e_ren {M Γ1 Γ2 Γ3} (u : Γ2 ⊆ Γ3) (v : Γ1 =[M.(val)]> Γ2)
-             : Γ1 =[M.(val)]> Γ3
-    := e_comp (s_ren M.(v_var) u) v.
+  Definition e_ren {Γ1 Γ2 Γ3} : Γ2 ⊆ Γ3 -> Γ1 ⇒ᵥ Γ2 -> Γ1 ⇒ᵥ Γ3
+    := fun u v => (v_var ⊛ᵣ u) ⊛ v.
+  Infix "⊛ᵣ'" := e_ren (at level 14).
 
-  Definition c_ren {M Γ1 Γ2} (u : Γ1 ⊆ Γ2) (c : M.(conf) Γ1) : M.(conf) Γ2
-    := M.(c_sub) (e_ren u M.(v_var)) c.
+  Definition c_ren {Γ1 Γ2} : Γ1 ⊆ Γ2 -> conf Γ1 -> conf Γ2
+    := fun u c => (u ⊛ᵣ' v_var) @ₜ c.
 
-  Class machine_law (M : machine) : Prop := {
+  Class machine_law : Prop := {
     v_sub_proper {Γ Δ}
       :> Proper
           (sub_eq Γ Δ ==> forall_relation (fun i => eq ==> eq))
-          M.(v_sub) ;
+          v_sub ;
     c_sub_proper {Γ Δ}
       :> Proper
           (sub_eq Γ Δ ==> eq ==> eq)
-          M.(c_sub) ;
-    v_sub_var {Γ1 Γ2} (p : Γ1 =[M.(val)]> Γ2)
-      : sub_eq _ _ (e_comp p M.(v_var)) p ;
-    v_var_sub {Γ1 Γ2} (p : Γ1 =[M.(val)]> Γ2)
-      : sub_eq _ _ (e_comp M.(v_var) p) p ;
-    v_sub_sub {Γ1 Γ2 Γ3 Γ4}
-      (p : Γ3 =[M.(val)]> Γ4) (q : Γ2 =[M.(val)]> Γ3) (r : Γ1 =[M.(val)]> Γ2)
-      : sub_eq _ _ (e_comp p (e_comp q r)) (e_comp (e_comp p q) r) ;
-    c_var_sub {Γ} (c : M.(conf) Γ)
-      : M.(c_sub) M.(v_var) c
-      = c ;
-    c_sub_sub {Γ1 Γ2 Γ3} (u : Γ2 =[M.(val)]> Γ3) (v : Γ1 =[M.(val)]> Γ2) {c}
-      : M.(c_sub) u (M.(c_sub) v c)
-      = M.(c_sub) (e_comp u v) c ;
-  }. 
-  Arguments c_sub_proper {M}.
-  Arguments v_sub_proper {M}.
-  Arguments v_sub_var {M}.
-  Arguments v_var_sub {M}.
-  Arguments v_sub_sub {M}.
-  Arguments c_var_sub {M}.
-  Arguments c_sub_sub {M}.
+          c_sub ;
+    v_sub_var {Γ1 Γ2} (p : Γ1 ⇒ᵥ Γ2) : p ⊛ v_var ≡ₛ p ;
+    v_var_sub {Γ1 Γ2} (p : Γ1 ⇒ᵥ Γ2) : v_var ⊛ p ≡ₛ p ;
+    v_sub_sub {Γ1 Γ2 Γ3 Γ4} (p : Γ3 ⇒ᵥ Γ4) (q : Γ2 ⇒ᵥ Γ3) (r : Γ1 ⇒ᵥ Γ2)
+      : p ⊛ (q ⊛ r) ≡ₛ (p ⊛ q) ⊛ r ;
+    c_var_sub {Γ} (c : conf Γ) : v_var @ₜ c = c ;
+    c_sub_sub {Γ1 Γ2 Γ3} (u : Γ2 ⇒ᵥ Γ3) (v : Γ1 ⇒ᵥ Γ2) {c}
+      : u @ₜ (v @ₜ c) = (u ⊛ v) @ₜ c ;
+  }.
 
-  #[global] Instance e_comp_proper {M} {MH : machine_law M} {Γ1 Γ2 Γ3}
-             : Proper (sub_eq Γ2 Γ3 ==> sub_eq Γ1 Γ2 ==> sub_eq Γ1 Γ3) (@e_comp M _ _ _).
+  Context {MH : machine_law}.
+
+  #[global] Instance e_comp_proper {Γ1 Γ2 Γ3}
+             : Proper (sub_eq Γ2 Γ3 ==> sub_eq Γ1 Γ2 ==> sub_eq Γ1 Γ3) e_comp.
     intros ? ? H1 ? ? H2 ? i.
     unfold e_comp, s_map.
     now rewrite H1, H2.
   Qed.
 
-  #[global] Instance e_ren_proper {M} {MH : machine_law M} {Γ1 Γ2 Γ3}
-             : Proper (sub_eq Γ2 Γ3 ==> sub_eq Γ1 Γ2 ==> sub_eq Γ1 Γ3) (@e_ren M _ _ _).
+  #[global] Instance e_ren_proper {Γ1 Γ2 Γ3}
+             : Proper (sub_eq Γ2 Γ3 ==> sub_eq Γ1 Γ2 ==> sub_eq Γ1 Γ3) e_ren.
   intros ? ? H1 ? ? H2.
   unfold e_ren. apply e_comp_proper; eauto. now rewrite H1.
   Qed.
 
-  Lemma e_comp_ren_r {M Γ1 Γ2 Γ3 Γ4} (u : env M Γ3 Γ4) (v : env M Γ2 Γ3) (w : Γ1 ⊆ Γ2) :
-    sub_eq _ _ (e_comp u (s_ren v w)) (s_ren (e_comp u v) w) .
+  Lemma e_comp_ren_r {Γ1 Γ2 Γ3 Γ4} (u : Γ3 ⇒ᵥ Γ4) (v : Γ2 ⇒ᵥ Γ3) (w : Γ1 ⊆ Γ2)
+        : u ⊛ (v ⊛ᵣ w) ≡ₛ (u ⊛ v) ⊛ᵣ w .
     reflexivity.
   Qed.
 
-  Lemma e_comp_ren_l {M} {MH : machine_law M} {Γ1 Γ2 Γ3 Γ4} (u : env M Γ3 Γ4) (v : Γ2 ⊆ Γ3) (w : env M Γ1 Γ2) :
-    sub_eq _ _ (e_comp (s_ren u v) w) (e_comp u (e_ren v w)) .
+  Lemma e_comp_ren_l {Γ1 Γ2 Γ3 Γ4} (u : Γ3 ⇒ᵥ Γ4) (v : Γ2 ⊆ Γ3) (w : Γ1 ⇒ᵥ Γ2)
+        : (u ⊛ᵣ v) ⊛ w ≡ₛ u ⊛ (v ⊛ᵣ' w) .
     unfold e_ren.
-    now rewrite MH.(v_sub_sub), e_comp_ren_r, MH.(v_sub_var).
+    now rewrite v_sub_sub, e_comp_ren_r, v_sub_var.
   Qed.
 
-  Program Definition sub_eval_msg {Γ Δ} (M : machine) (e : Γ =[M.(val)]> Δ) (t : M.(conf) Γ)
+  Program Definition sub_eval_msg {Γ Δ} (e : Γ ⇒ᵥ Δ) (t : conf Γ)
              : delay (msg' Δ)
-    := fmap (fun _ => @projT1 _ _) _ (M.(eval) (M.(c_sub) e t)).
+    := fmap (fun _ => @projT1 _ _) _ (eval (e @ₜ t)).
 
-  #[global] Instance sub_eval_msg_proper {Γ Δ} {M : machine} {MH : machine_law M}
-             : Proper (sub_eq Γ Δ ==> pointwise_relation _ eq) (@sub_eval_msg Γ Δ M).
+  #[global] Instance sub_eval_msg_proper {Γ Δ}
+             : Proper (sub_eq Γ Δ ==> pointwise_relation _ eq) (@sub_eval_msg Γ Δ).
   Proof.
     intros ? ? H1 e.
     unfold sub_eval_msg.
     now rewrite H1.
   Qed.
 
-  Definition ciu (M : machine) {Γ} Δ (x y : M.(conf) Γ) : Prop :=
-    forall (e : Γ =[M.(val)]> Δ), it_wbisim (sub_eval_msg M e x) (sub_eval_msg M e y).
+  Definition ciu {Γ} Δ (x y : conf Γ) : Prop :=
+    forall (e : Γ ⇒ᵥ Δ), it_wbisim (sub_eval_msg e x) (sub_eval_msg e y).
 
   (* Section 3: game definition
      ↓+ ~ join_even
    *)
   Definition alt_ext : Type := ctx (ctx S.(typ)).
+  Notation "↓⁺ a" := (join_even a) (at level 9).
+  Notation "↓⁻ a" := (join_odd a) (at level 9).
+  Notation "↓[ b ] a" := (join_even_odd_aux b a) (at level 9).
+
 
   Definition ogs_hg : half_game alt_ext alt_ext := {|
-    g_move := fun es => msg' (join_even es) ;
+    g_move := fun es => msg' ↓⁺es ;
     g_next := fun es m => (es ▶ dom' m) ;
   |}.
 
@@ -171,107 +170,72 @@ TODO: concretize env
      Env M Δ player es : environment part of the player (aka active at es) configuration at (Δ + es)
      Env M Δ opponent es : environment part of the opponent (aka passive at es) configuration at (Δ + es)
    *)
-  Inductive alt_env (M : machine) (Δ : ctx S.(typ))
+  Inductive alt_env (Δ : ctx S.(typ))
     : bool -> alt_ext -> Type :=
-  | ENil {b} : alt_env M Δ b ∅
-  | EConT {a Γ} : alt_env M Δ opponent a
-                  -> alt_env M Δ player (a ▶ Γ)
-  | EConF {a Γ} : alt_env M Δ player a
-                  -> Γ =[M.(val)]> (Δ +▶ join_even a)
-                  -> alt_env M Δ opponent (a ▶ Γ)
+  | ENil {b} : alt_env Δ b ∅
+  | EConT {a Γ} : alt_env Δ opponent a
+                  -> alt_env Δ player (a ▶ Γ)
+  | EConF {a Γ} : alt_env Δ player a
+                  -> Γ ⇒ᵥ (Δ +▶ ↓⁺a)
+                  -> alt_env Δ opponent (a ▶ Γ)
   .
-  Arguments ENil {M Δ b}.
-  Arguments EConT {M Δ a Γ}.
-  Arguments EConF {M Δ a Γ}.
+  Arguments ENil {Δ b}.
+  Arguments EConT {Δ a Γ}.
+  Arguments EConF {Δ a Γ}.
 
   (* flattens an alternating environment into an unstructured one *)
-  Equations concat0 {M Δ b a} : alt_env M Δ b a
-             -> (join_even_odd_aux (negb b) a) =[M.(val)]> (Δ +▶ join_even_odd_aux b a) :=
+  Equations concat0 {Δ b a} : alt_env Δ b a -> ↓[negb b] a ⇒ᵥ (Δ +▶ ↓[b] a) :=
     concat0 (ENil) := s_empty ;
-    concat0 (EConT u) := e_ren r_concat3_1 (concat0 u) ;
-    concat0 (EConF u e) := s_cat (concat0 u) e .
+    concat0 (EConT u) := r_concat3_1 ⊛ᵣ' concat0 u ;
+    concat0 (EConF u e) := [ concat0 u , e ] .
 
   (* Flattens a pair of alternating environments for resp. player and opponent into a "closed" substitution *)
-  Equations concat1 {M Δ} a b :
-    alt_env M Δ b a ->
-    alt_env M Δ (negb b) a ->
-    (join_even_odd_aux b a) =[M.(val)]> Δ :=
+  Equations concat1 {Δ} a b : alt_env Δ b a -> alt_env Δ (negb b) a -> ↓[b] a ⇒ᵥ Δ :=
     concat1 ∅      b _ _ :=
       s_empty ;
     concat1 (a ▶ _) b (EConT u) (EConF v e) :=
-      s_cat
-        (concat1 a _ u v)
-        (e_comp (s_cat M.(v_var) (concat1 a _ v u)) e) ;
+      [ concat1 a _ u v , [ v_var , concat1 a _ v u ] ⊛ e ] ;
     concat1 (a ▶ _) b (EConF u e) (EConT v) := concat1 a _ u v .
-  Arguments concat1 {M Δ a}.
+  Arguments concat1 {Δ a b}.
 
-  Lemma quatre_six {M} {MH : machine_law M} {Δ a}
-    (u : alt_env M Δ player a) (v : alt_env M Δ opponent a)
-    : sub_eq _ _ (e_comp (s_cat M.(v_var) (concat1 player u v)) (concat0 u))
-                 (concat1 opponent v u) 
-    /\ sub_eq _ _ (e_comp (s_cat M.(v_var) (concat1 opponent v u)) (concat0 v))
-                  (concat1 player u v) .
+  Lemma quatre_six {Δ a} (u : alt_env Δ player a) (v : alt_env Δ opponent a)
+    :  [ v_var , concat1 u v ] ⊛ concat0 u ≡ₛ concat1 v u
+    /\ [ v_var , concat1 v u ] ⊛ concat0 v ≡ₛ concat1 u v .
+    (*
     induction a; dependent destruction u; dependent destruction v; cbn; split.
     - intros ? i; dependent elimination i.
     - intros ? i; dependent elimination i.
+    - unfold s_cat. rewrite s_cover_assoc.
     - unfold r_concat3_1.
       unfold e_ren.
-      rewrite MH.(v_sub_sub).
+      rewrite v_sub_sub.
       rewrite e_comp_ren_r.
-      rewrite MH.(v_sub_var).
-      Admitted.
-(*      rewrite s_eq_cat_l.
-      rewrite (proj2 (IHa v u)).
-      rewrite (proj1 (IHa v u)).
-      unfold e_ren.
-      Search s_ren.
-      unfold e_ren.
-      rewrite MH.(v_sub_sub).
-      rewrite e_comp_ren_r.
-      rewrite MH.(v_sub_var).
-      rewrite e_comp_ren_l.
-      Search s_ren.
-      rewrite 
-    
-    cbn.
-    Search s_empty.
-    rewrite s_eq_cover_empty_r.
-        
-    {x i} :
-    e_comp
-        (s_cat M.(v_var) (concat1 b u v))
-        (concat0 u) x i
-    = concat1 (negb b)
-        v
-        (rew [fun x => alt_env _ _ x _] (Bool.negb_involutive_reverse b) in u)
-        x i.
-  Admitted.
+      rewrite v_sub_var.
 *)
+      Admitted.
 
-  Definition m_strat_act (M : machine) Δ : alt_ext -> Type :=
-    fun a => (M.(conf) (Δ +▶ join_even a) * alt_env M Δ player a)%type.
+  Definition m_strat_act Δ : alt_ext -> Type :=
+    fun a => (conf (Δ +▶ join_even a) * alt_env Δ player a)%type.
 
-  Definition m_strat_pas (M : machine) Δ : alt_ext -> Type :=
-    fun a => alt_env M Δ opponent a.
+  Definition m_strat_pas Δ : alt_ext -> Type :=
+    fun a => alt_env Δ opponent a.
 
-  Definition m_strat_play {M Δ a} (x : m_strat_act M Δ a)
-    : delay (msg' Δ + h_actv ogs_hg (m_strat_pas M Δ) a)%type :=
-    (M.(eval) (fst x)) >>=
+  Definition m_strat_play {Δ a} (x : m_strat_act Δ a)
+    : delay (msg' Δ + h_actv ogs_hg (m_strat_pas Δ) a)%type :=
+    (eval (fst x)) >>=
       fun _ u =>
-        match cover_split cover_cat (fst (projT2 (projT1 u))) with
+        match cover_split cover_cat _ (fst (projT2 (projT1 u))) with
         | inl h => Ret' (inl (_ ,' (h , snd (projT2 (projT1 u)))))
         | inr h => Ret' (inr ((_ ,' (h , snd (projT2 (projT1 u)))) ,' EConF (snd x) (projT2 u)))
         end .
 
-  Definition m_strat_resp {M Δ a} (x : m_strat_pas M Δ a)
-    : h_pasv ogs_hg (m_strat_act M Δ) a
-    := fun m => (M.(c_sub)
-                  (s_cat (e_ren r_concat3_1 (concat0 x))
-                         (e_ren (r_concat_r ∘⊆ r_concat_r) M.(v_var)))
-              (M.(emb) m) ,
+  Definition m_strat_resp {Δ a} (x : m_strat_pas Δ a)
+    : h_pasv ogs_hg (m_strat_act Δ) a
+    := fun m =>
+         ([ (r_concat3_1 ⊛ᵣ' concat0 x) , (r_concat_r ∘⊆ r_concat_r) ⊛ᵣ' v_var ] @ₜ emb m ,
           EConT x).
 
-  Definition m_strat {M Δ} : m_strat_act M Δ ⇒ᵢ itree ogs_e (fun _ => msg' Δ) :=
+  Definition m_strat {Δ} : m_strat_act Δ ⇒ᵢ itree ogs_e (fun _ => msg' Δ) :=
     iter
       (fun i e =>
          emb_delay (m_strat_play e) >>=
@@ -281,21 +245,19 @@ TODO: concretize env
              | inr (m,'c) => Vis' (m : ogs_e.(e_qry) i) (fun r => Ret' (inl (m_strat_resp c r)))
              end).
 
-  Definition m_stratp {M Δ} : m_strat_pas M Δ ⇒ᵢ h_pasv ogs_hg (itree ogs_e (fun _ => msg' Δ)) :=
+  Definition m_stratp {Δ} : m_strat_pas Δ ⇒ᵢ h_pasv ogs_hg (itree ogs_e (fun _ => msg' Δ)) :=
     fun _ x m => m_strat _ (m_strat_resp x m).
 
-  Definition inj_init_act {M : machine} {Δ Γ} (c : M.(conf) Γ)
-             : m_strat_act M Δ (∅ ▶ Γ)
+  Definition inj_init_act {Δ Γ} (c : conf Γ) : m_strat_act Δ (∅ ▶ Γ)
     := (c_ren (r_concat_r ∘⊆ r_concat_r) c , EConT ENil).
 
-  Definition inj_init_pas {M : machine} {Δ Γ} (γ : Γ =[M.(val)]> Δ)
-             : m_strat_pas M Δ (∅ ▶ Γ)
+  Definition inj_init_pas {Δ Γ} (γ : Γ ⇒ᵥ Δ) : m_strat_pas Δ (∅ ▶ Γ)
     := EConF ENil (e_ren r_concat_l γ).
 
-  Definition compo_t M (Δ : ctx S.(typ)) : Type := ⦉ m_strat_act M Δ ×ᵢ m_strat_pas M Δ ⦊ᵢ .
+  Definition compo_t (Δ : ctx S.(typ)) : Type := ⦉ m_strat_act Δ ×ᵢ m_strat_pas Δ ⦊ᵢ .
 
-  Equations compo_body {M Δ} : (fun (_ : T1) => compo_t M Δ)
-                             ⇒ᵢ itree ∅ₑ (fun _ => compo_t M Δ + msg' Δ)%type :=
+  Equations compo_body {Δ}
+            : (fun (_ : T1) => compo_t Δ) ⇒ᵢ itree ∅ₑ (fun _ => compo_t Δ + msg' Δ)%type :=
     compo_body T1_0 x :=
       m_strat_play (fst (projT2 x)) >>= fun _ r =>
           go (match r with
@@ -303,30 +265,30 @@ TODO: concretize env
               | inr e => RetF (inl (_ ,' (m_strat_resp (snd (projT2 x)) (projT1 e) , (projT2 e))))
               end).  
 
-  Definition compo {M Δ} a
-    (u : m_strat_act M Δ a)
-    (v : m_strat_pas M Δ a)
-    : delay (msg' Δ)
+  Definition compo {Δ a} (u : m_strat_act Δ a) (v : m_strat_pas Δ a) : delay (msg' Δ)
     := iter compo_body T1_0 (a ,' (u , v)).
 
+  Notation "u ∥ v" := (compo u v) (at level 40).
+
   (* guilhem: rename? *)
-  Definition barb (M : machine) {Γ} Δ (x y : M.(conf) Γ) : Prop :=
-    forall e : Γ =[M.(val)]> Δ,
-    it_wbisim (compo _ (inj_init_act x) (inj_init_pas e))
-              (compo _ (inj_init_act y) (inj_init_pas e)).
+  Definition barb {Γ} Δ (x y : conf Γ) : Prop :=
+    forall e : Γ ⇒ᵥ Δ,
+    it_wbisim (inj_init_act x ∥ inj_init_pas e) (inj_init_act y ∥ inj_init_pas e).
 
-  Equations reduce {M : machine} {Δ} : (fun (_ : T1) => compo_t M Δ) ⇒ᵢ itree ∅ₑ (fun _ => msg' Δ) :=
-    reduce T1_0 u := sub_eval_msg M (s_cat (M.(v_var)) (concat1 _ (snd (fst (projT2 u))) (snd (projT2 u)))) (fst (fst (projT2 u))) .
+  Equations reduce {Δ} : (fun (_ : T1) => compo_t Δ) ⇒ᵢ itree ∅ₑ (fun _ => msg' Δ) :=
+    reduce T1_0 u := sub_eval_msg
+                       ([ v_var , concat1 (snd (fst (projT2 u))) (snd (projT2 u)) ])
+                       (fst (fst (projT2 u))) .
 
-  Lemma quatre_trois_pre {M : machine} {Δ} (x : compo_t M Δ)
+  Lemma quatre_trois_pre {Δ} (x : compo_t Δ)
     : it_eq
         (compo_body T1_0 x >>= fun _ r => go (match r with
                                      | inl x' => TauF (reduce _ x')
                                      | inr y => RetF (y : (fun _ => msg' _) _)
                                      end))
-      (M.(eval) (fst (fst (projT2 x))) >>=
+      (eval (fst (fst (projT2 x))) >>=
                       fun _ u =>
-                        go (match cover_split cover_cat (fst (projT2 (projT1 u))) with
+                        go (match cover_split cover_cat _ (fst (projT2 (projT1 u))) with
                             | inl h => RetF (_ ,' (h, snd (projT2 (projT1 u))))
                             | inr h => TauF (reduce _ (_ ,'
                                                     (m_strat_resp (snd (projT2 x)) (_ ,' (h, snd (projT2 (projT1 u)))), EConF (snd (fst (projT2 x))) (projT2 u))))
@@ -336,41 +298,39 @@ TODO: concretize env
     unfold compo_body; apply bind_bind_com.
     etransitivity.
     unfold m_strat_play; apply bind_bind_com.
-    remember (M.(eval) (fst (fst (projT2 x)))) as t eqn:H; clear H; revert t.
+    remember (eval (fst (fst (projT2 x)))) as t eqn:H; clear H; revert t.
     unfold it_eq; coinduction R CIH; intros t.
     cbn; destruct (t.(_observe)).
     + destruct r as [[? [i m]] γ]; cbn.
-      destruct (cover_split cover_cat i).
+      destruct (cover_split cover_cat _ i).
       econstructor; reflexivity.
       econstructor; reflexivity.
     + econstructor. apply CIH.
     + destruct q.
   Qed.
     
-  Definition eval_sub_1 {M : machine} {Γ Δ} (c : M.(conf) (Δ +▶ Γ)) (e : Γ =[M.(val)]> Δ)
-             : delay { m : msg' Δ & dom' m =[M.(val)]> Δ } :=
-        M.(eval) (M.(c_sub) (s_cat M.(v_var) e) c) .
+  Definition eval_sub_1 {Γ Δ} (c : conf (Δ +▶ Γ)) (e : Γ ⇒ᵥ Δ)
+             : delay { m : msg' Δ & dom' m ⇒ᵥ Δ } :=
+        eval ([ v_var , e ] @ₜ c) .
 
-  Definition eval_sub_2 {M : machine} {Γ Δ} (c : M.(conf) (Δ +▶ Γ)) (e : Γ =[M.(val)]> Δ)
-             : delay { m : msg' Δ & dom' m =[M.(val)]> Δ }.
-    refine (M.(eval) c >>= fun 'T1_0 x =>
-               go (match cover_split cover_cat (fst (projT2 (projT1 x))) with
+  Definition eval_sub_2 {Γ Δ} (c : conf (Δ +▶ Γ)) (e : Γ ⇒ᵥ Δ)
+             : delay { m : msg' Δ & dom' m ⇒ᵥ Δ }.
+    refine (eval c >>= fun 'T1_0 x =>
+               go (match cover_split cover_cat _ (fst (projT2 (projT1 x))) with
                    | inl h => RetF ((_ ,' (h , snd (projT2 (projT1 x)))) ,'
-                                   e_comp (s_cat M.(v_var) e) (projT2 x))
+                                   [ v_var,  e ] ⊛ (projT2 x))
                    | inr h => TauF _
                    end)) .
-    refine (M.(eval) (M.(c_sub) (s_cat e (e_comp (s_cat M.(v_var) e) (projT2 x))) (M.(emb) (_ ,' (h , (snd (projT2 (projT1 x)))))))).
+    refine (eval ([ e , ([v_var , e ] ⊛ projT2 x) ] @ₜ (emb (_ ,' (h , (snd (projT2 (projT1 x)))))))).
   Defined.
 
-  Hypothesis eval_hyp : forall {M : machine} {Γ Δ}
-                          (c : M.(conf) (Δ +▶ Γ))
-                          (e : Γ =[M.(val)]> Δ),
+  Hypothesis eval_hyp : forall {Γ Δ}
+                          (c : conf (Δ +▶ Γ))
+                          (e : Γ ⇒ᵥ Δ),
                           it_eq (eval_sub_1 c e) (eval_sub_2 c e) .
 
-  Lemma quatre_trois {M : machine} {MH : machine_law M} {Δ a}
-    (c : m_strat_act M Δ a)
-    (e : m_strat_pas M Δ a)
-    : it_eq (reduce _ (_ ,' (c , e))) (compo _ c e) .
+  Lemma quatre_trois {Δ a} (c : m_strat_act Δ a) (e : m_strat_pas Δ a)
+    : it_eq (reduce _ (_ ,' (c , e))) (c ∥ e) .
     refine (iter_lem compo_body reduce _ _ (_ ,' (c , e))).
     clear a c e; intros [] [ ? [ u v ] ].
     etransitivity; cycle 1.
@@ -382,41 +342,49 @@ TODO: concretize env
     apply bind_fmap_com.
     unfold it_eq; cbn [fst snd projT2 projT1].
     apply (tt_t (it_eq_map ∅ₑ (fun _ : T1 => msg' Δ))).
-    refine (@it_eq_up2bind_t _ ∅ₑ (fun _ => {m : msg' (Δ +▶ join_even x) & dom' m =[ val M ]> (Δ +▶ join_even x)}) _ _ _ (M.(eval) (fst u) >>= _) (M.(eval) (fst u) >>= _) _).
+    refine (@it_eq_up2bind_t _ ∅ₑ (fun _ => {m : msg' (Δ +▶ join_even x) & dom' m ⇒ᵥ (Δ +▶ _)}) _ _ _ (eval (fst u) >>= _) (eval (fst u) >>= _) _).
     econstructor; eauto.
     intros [] [m γ].
     apply (bt_t (it_eq_map ∅ₑ (fun _ : T1 => msg' Δ))).
     cbn [fst snd projT2 projT1].
-    destruct (cover_split cover_cat (fst (projT2 m))).
+    destruct (cover_split cover_cat _ (fst (projT2 m))).
     - econstructor.
     - econstructor.
       unfold reduce.
-      fold (@fmap _ ∅ₑ _ _ (fun _ : T1 => projT1 (P:=fun m0 : msg' Δ => dom' m0 =[ val M ]> Δ)) T1_0).
+      fold (@fmap _ ∅ₑ _ _ (fun _ : T1 => projT1 (P:=fun m0 : msg' Δ => dom' m0 ⇒ᵥ Δ)) T1_0).
       change (it_eq_t ∅ₑ (fun _ : T1 => msg' Δ) bot T1_0 ?a ?b) with (it_eq a b).
       apply fmap_eq.
       unfold m_strat_resp.
       cbn [fst snd projT1 projT2].
-      rewrite MH.(c_sub_sub).
-      unshelve rewrite MH.(c_sub_proper); try reflexivity.
+      rewrite c_sub_sub.
+      unshelve rewrite c_sub_proper; try reflexivity.
   Admitted.
 
-  Lemma quatre_trois_app {M : machine} {MH : machine_law M} {Γ Δ}
-    (c : M.(conf) Γ) (e : Γ =[M.(val)]> Δ)
-    : it_eq (sub_eval_msg M e c) (compo _ (inj_init_act c) (inj_init_pas e)).
+  Lemma quatre_trois_app {Γ Δ}
+    (c : conf Γ) (e : Γ ⇒ᵥ Δ)
+    : it_eq (sub_eval_msg e c) (inj_init_act c ∥ inj_init_pas e).
   Proof.
     rewrite <- quatre_trois.
     unfold reduce, inj_init_act, sub_eval_msg; cbn [fst snd projT1 projT2]; apply fmap_eq.
     cbv [inj_init_pas]; rewrite concat1_equation_2, 2 concat1_equation_1.
-    unfold c_ren; rewrite MH.(c_sub_sub), MH.(c_sub_proper) ; try reflexivity.
-    unfold e_ren; rewrite MH.(v_sub_sub), MH.(v_sub_var).
-    rewrite s_eq_cover_empty_r, e_comp_ren_r, MH.(v_sub_var), s_ren_comp.
+    unfold c_ren; rewrite c_sub_sub, c_sub_proper ; try reflexivity.
+    unfold e_ren; rewrite v_sub_sub, v_sub_var.
+    rewrite s_eq_cover_empty_r.
+    (*
+    rewrite v_var_sub.
+    rewrite s_eq_cover_empty_r, e_comp_ren_r, v_sub_var, s_ren_comp.
+    rewrite e_comp_ren_r.
+    rewrite e_comp_ren_r.
+    rewrite v_sub_var.
     rewrite 2 s_eq_cat_r.
     unfold r_concat_l, cover_cat; cbn; rewrite r_cover_l_nil.
-    now rewrite 2 MH.(v_var_sub).
+    now rewrite 2 v_var_sub.
   Qed.
+*)
+    Admitted.
 
-  Theorem ogs_correction (M : machine) (MH : machine_law M) {Γ} Δ (x y : M.(conf) Γ)
-          : barb M Δ x y -> ciu M Δ x y.
+  Theorem ogs_correction {Γ} Δ (x y : conf Γ)
+          : barb Δ x y -> ciu Δ x y.
   Proof.
     intros H e.
     etransitivity; [ apply it_eq_wbisim, (quatre_trois_app x e) | ].
